Support "diving into" blocks to find code. See msg.
Previously, we required both the original code and the hint to have an
equivalent set of blocks. Now instead, we allow the original code to
be deeper. The hint needs to be shallower and is used to decide how to
"dive into" the original code to find the relevant code.

The reason it is ok to not "break apart" the hint when diving in is
because the expected use case will only be a logical reordering of the
code, and not an arbitrary reordering. In this case, either we will
have the necessary blocks already, or we want to be at the level of
instructions, but in that case, we already will have those at the
hint.

vale/code/lib/transformers/Vale.Transformers.InstructionReorder.fst
@@ -1563,9 +1563,23 @@ let rec bubble_to_top (cs:codes) (i:nat{i < L.length cs}) : possibly (cs':codes{
     )
 #pop-options
 
+let rec num_blocks_in_codes (c:codes) : nat =
+  match c with
+  | [] -> 0
+  | Block l :: t -> 1 + num_blocks_in_codes l + num_blocks_in_codes t
+  | _ :: t -> num_blocks_in_codes t
+
+let rec lemma_num_blocks_in_codes_append (c1 c2:codes) :
+  Lemma
+    (ensures (num_blocks_in_codes (c1 `L.append` c2) == num_blocks_in_codes c1 + num_blocks_in_codes c2))
+    [SMTPat (num_blocks_in_codes (c1 `L.append` c2))] =
+  match c1 with
+  | [] -> ()
+  | x :: xs -> lemma_num_blocks_in_codes_append xs c2
+
 let rec reordering_allowed (c1 c2 : codes) :
   Tot pbool
-    (decreases %[c2]) =
+    (decreases %[c2; num_blocks_in_codes c1]) =
   match c1, c2 with
   | [], [] -> ttrue
   | [], _ | _, [] -> ffalse "disagreeing lengths of codes"
@@ -1580,6 +1594,9 @@ let rec reordering_allowed (c1 c2 : codes) :
         match h1, h2 with
         | Block l1, Block l2 ->
           reordering_allowed l1 l2 &&. reordering_allowed t1 t2
+        | Block l1, _ -> (
+            reordering_allowed (l1 `L.append` t1) c2
+          )
         | _ -> Err reason (* TODO: Handle IfElse and While specially too? *)
       )
 
@@ -1588,7 +1605,7 @@ let rec perform_reordering (c1 c2 : codes) :
   Pure (codes)
     (requires !!(reordering_allowed c1 c2))
     (ensures (fun c_gen -> eq_codes c_gen c2))
-    (decreases %[c2]) =
+    (decreases %[c2; num_blocks_in_codes c1]) =
   match c1, c2 with
   | [], [] -> []
   | _, h2 :: t2 ->
@@ -1603,6 +1620,8 @@ let rec perform_reordering (c1 c2 : codes) :
         | Block l1, Block l2 ->
           assert (eq_code (Block (perform_reordering l1 l2)) (Block l2)); (* OBSERVE *)
           Block (perform_reordering l1 l2) :: perform_reordering t1 t2
+        | Block l1, _ ->
+          perform_reordering (l1 `L.append` t1) c2
       )
 
 /// If there are two sequences of instructions that can be transformed
@@ -1645,6 +1664,19 @@ let rec lemma_bubble_to_top (cs : codes) (i:nat{i < L.length cs}) (fuel:nat) (s 
     )
 #pop-options
 
+#push-options "--initial_fuel 3 --max_fuel 3 --initial_ifuel 1 --max_ifuel 1"
+let rec lemma_machine_eval_codes_block_to_append (c1 c2 : codes) (fuel:nat) (s:machine_state) :
+  Lemma
+    (ensures (machine_eval_codes (c1 `L.append` c2) fuel s == machine_eval_codes (Block c1 :: c2) fuel s)) =
+  match c1 with
+  | [] -> ()
+  | x :: xs ->
+    match machine_eval_code x fuel s with
+    | None -> ()
+    | Some s1 ->
+      lemma_machine_eval_codes_block_to_append xs c2 fuel s1
+#pop-options
+
 let rec lemma_reordering (c1 c2 : codes) (fuel:nat) (s1 : machine_state) :
   Lemma
     (requires (
@@ -1657,7 +1689,7 @@ let rec lemma_reordering (c1 c2 : codes) (fuel:nat) (s1 : machine_state) :
            machine_eval_codes c1 fuel s1,
            machine_eval_codes (perform_reordering c1 c2) fuel s1 in
          equiv_states_or_both_not_ok s1' s2')))
-    (decreases %[c2]) =
+    (decreases %[c2; num_blocks_in_codes c1]) =
   match c2 with
   | [] -> ()
   | h2 :: t2 ->
@@ -1696,4 +1728,7 @@ let rec lemma_reordering (c1 c2 : codes) (fuel:nat) (s1 : machine_state) :
           assert (equiv_states s2' s2'');
           assert (machine_eval_codes (perform_reordering c1 c2) fuel s1 == machine_eval_codes (perform_reordering t1 t2) fuel s1'');
           assert (Some s2'' == machine_eval_codes (perform_reordering c1 c2) fuel s1)
+        | Block l1, _ ->
+          lemma_machine_eval_codes_block_to_append l1 t1 fuel s1;
+          lemma_reordering (l1 `L.append` t1) c2 fuel s1
       )
